Blake3/C.lean
@@ -1,0 +1,49 @@
+import Blake3
+/-! C-backed BLAKE3 bindings. -/
+
+namespace Blake3.C
+open Blake3
+public section
+
+private opaque HasherNonempty : NonemptyType
+
+def Hasher : Type := HasherNonempty.type
+
+instance : Nonempty Hasher := HasherNonempty.property
+
+@[extern "c_blake3_version"]
+protected opaque internalVersion : Unit → String
+
+/-- Version of the linked C BLAKE3 implementation library. -/
+def version : String := Blake3.C.internalVersion ()
+
+@[extern "c_blake3_init"]
+private opaque hasherInit : Unit → Hasher
+
+@[extern "c_blake3_init_keyed"]
+private opaque hasherInitKeyed : @& Blake3Key → Hasher
+
+@[extern "c_blake3_init_derive_key"]
+private opaque hasherInitDeriveKey : @& ByteArray → Hasher
+
+@[extern "c_blake3_hasher_update"]
+private opaque hasherUpdate : Hasher → @& ByteArray → Hasher
+
+@[extern "c_blake3_hasher_finalize"]
+private opaque hasherFinalize : Hasher → (length : USize) →
+  { r : ByteArray // r.size = length.toNat }
+
+instance : HasherOps Hasher where
+  init := hasherInit
+  initKeyed := hasherInitKeyed
+  initDeriveKey := hasherInitDeriveKey
+  update := hasherUpdate
+  finalize := hasherFinalize
+
+abbrev hash := HasherOps.hash (H := Hasher)
+abbrev hashKeyed := HasherOps.hashKeyed (H := Hasher)
+abbrev hashDeriveKey := HasherOps.hashDeriveKey (H := Hasher)
+abbrev Sponge := Blake3.Sponge Hasher
+
+end
+end Blake3.C
